Monadic lens induces lens algebra for stateT

Related.v
@@ -1,4 +1,77 @@
 Require Import Background.
+Require Import Towards.
+
+
+(* stateT *)
+
+Record stateT (S : Type) (m : Type -> Type) `{Monad m} (A : Type) := mkStateT
+{ runStateT : S -> m (A * S)%type }.
+Arguments mkStateT [S m _ A].
+Arguments runStateT [S m _ A].
+
+Instance Monad_stateT (S : Type) (m : Type -> Type) 
+                     `{Monad m} : Monad (stateT S m) :=
+{ ret _ x       := mkStateT (fun s => ret (x, s))
+; bind _ _ mx f := mkStateT (fun s => runStateT mx s >>= 
+                                      (fun p => runStateT (f (fst p)) (snd p)))
+}.
+
+Instance MonadLaws_stateT (S : Type) (m : Type -> Type) 
+                         `{MonadLaws m} : MonadLaws (stateT S m).
+Proof.
+  destruct H0.
+  constructor; simpl; intros.
+  
+  - (* left id *)
+    rewrite (functional_extensionality_1
+      (fun s => ret (a, s) >>= (fun p : A * S => runStateT (f (fst p)) (snd p)))
+      (runStateT (f a))
+      (fun s => left_id _ _ _ _)).
+    destruct (f a).
+    now unwrap_layer.
+
+  - (* right id *)
+    destruct ma.
+    unwrap_layer.
+    simpl.
+    assert (G : forall A B (p : A * B), ret (fst p, snd p) = ret p).
+    { now destruct p. }
+    rewrite (monadic_extensionality_1 
+      (fun p => ret (fst p, snd p)) _ (fun _ => G _ _ _)).
+    now rewrite right_id.
+
+  - (* assoc *)
+    unwrap_layer.
+    auto.
+Qed.
+
+Instance MonadState_stateT (S : Type) (m : Type -> Type)
+                          `{Monad m} : MonadState S (stateT S m) :=
+{ get    := mkStateT (fun s => ret (s, s))
+; put s' := mkStateT (fun _ => ret (tt, s')) 
+}.
+
+Instance MonadStateLaws_stateT (S : Type) (m : Type -> Type)
+                              `{MonadLaws m} : MonadStateLaws S (stateT S m).
+Proof.
+  destruct H0.
+  constructor; simpl; intros.
+ 
+  - (* get_get *)
+    unwrap_layer.
+    now repeat rewrite left_id.
+
+  - (* get_put *)
+    unwrap_layer.
+    now rewrite left_id.
+
+  - (* put_get *)
+    now repeat rewrite left_id.
+
+  - (* put_put *)
+    now rewrite reta_gtgt_retb_is_retb.
+Qed.
+
 
 (* Monadic lenses *)
 
@@ -13,6 +86,60 @@ Arguments mkMLens [S A m _].
 Record mLensLaws {S A m} `{Monad m} (mln : mLens S A m) := mkMLensLaws
 { mview_mupdate : forall s, mupdate mln s (mview mln s) = ret s
 ; mupdate_mview : forall B (k : S -> A -> m B) s a, 
-                    mupdate mln s a >>= (fun s' => k s' (mview mln s')) =
-                    mupdate mln s a >>= (fun s' => k s' a)
+                         mupdate mln s a >>= (fun s' => k s' (mview mln s')) =
+                         mupdate mln s a >>= (fun s' => k s' a)
+  (* too much restrictive *)
+; mupdate_mupdate : forall s a1 a2,
+                           mupdate mln s a1 >>= (fun s' => mupdate mln s' a2) =
+                           mupdate mln s a2
 }.
+
+
+(* Connection between lens algebras and monadic lenses *)
+
+(* XXX: consider contemplating `Functor` to implement `update` *)
+Definition mLens_2_lensAlgStateT {S A m} `{Monad m}
+                                 (mln : mLens S A m) : lensAlg (stateT S m) A :=
+{| view      := mkStateT (fun s => ret (mview mln s, s))
+;  update a' := mkStateT (fun s => mupdate mln s a' >>= (fun s' => ret (tt, s')))
+|}.
+
+Theorem mLens_induces_lensAlgStateT : 
+    forall {S A m} `{MonadLaws m}
+           (mln : mLens S A m),
+           mLensLaws mln ->
+           lensAlgLaws (mLens_2_lensAlgStateT mln).
+Proof.
+  intros.
+  destruct H0.
+  destruct H1.
+  constructor; simpl; intros; unwrap_layer.
+
+  - (* get_get *)
+    now repeat rewrite left_id.
+
+  - (* get_put *)
+    rewrite left_id.
+    simpl.
+    rewrite mview_mupdate0.
+    now rewrite left_id.
+
+  - (* put_get *)
+    repeat rewrite assoc.
+    rewrite (monadic_extensionality_1
+      (fun s => ret (tt, s) >>= (fun p : unit * S => ret (mview mln (snd p), snd p)))
+      (fun s => ret (mview mln s, s))
+      (fun _ => left_id _ _ _ _)).
+    rewrite (mupdate_mview0 _ (fun s a => ret (a, s)) _ _).
+    unwrap_layer.
+    now rewrite left_id.
+
+  - (* put_put *)
+    rewrite assoc.
+    rewrite (monadic_extensionality_1
+      (fun s => ret (tt, s) >>= (fun p => mupdate mln (snd p) s2 >>= (fun s' => ret (tt, s'))))
+      (fun s => mupdate mln s s2 >>= (fun s' => ret (tt, s')))
+      (fun _ => left_id _ _ _ _)).
+    rewrite <- assoc.
+    now rewrite mupdate_mupdate0.
+Qed.
